ProofMining/FiniteType.lean
@@ -2,14 +2,7 @@
 inductive FiniteType where
 | zero : FiniteType
 | application : FiniteType → FiniteType → FiniteType
-<<<<<<< Updated upstream
 deriving Repr, DecidableEq, Inhabited
-=======
--- | void : FiniteType 
-deriving Repr, DecidableEq
-
--- instance : Inhabited FiniteType := ⟨FiniteType.void⟩
->>>>>>> Stashed changes
 
 notation "𝕆" => FiniteType.zero
 infixr:60 " ↣ " => FiniteType.application
@@ -17,10 +10,6 @@ infixr:60 " ↣ " => FiniteType.application
 def FiniteType.deg : FiniteType → Nat
   | FiniteType.zero => 0
   | FiniteType.application ρ τ => Nat.max (deg τ) ((deg ρ) + 1)
-<<<<<<< Updated upstream
-=======
-  -- | FiniteType.void => 0
->>>>>>> Stashed changes
 
 #eval FiniteType.deg (FiniteType.zero ↣ FiniteType.zero ↣ FiniteType.zero ↣ FiniteType.zero)
 
